

- Matrix Vector Multiplication

Want $\underline{x} \rightarrow \boxed{A} \rightarrow \underline{y} = A\underline{x}$ for $\underline{x} \in \mathbb{R}^n$
 $A \in \mathbb{R}^{m \times n}$
 $\underline{y} \in \mathbb{R}^m$

~~Inner~~ ^{Dot} Product View e.g.

$$\underline{y} = \underbrace{\begin{bmatrix} 1 & 2 & 3 \\ 4 & 5 & 6 \end{bmatrix}}_{\underline{A} \quad 2 \times 3} \underbrace{\begin{bmatrix} x_1 \\ x_2 \\ x_3 \end{bmatrix}}_{\underline{x} \quad 3 \times 1} = \begin{bmatrix} 1x_1 + 2x_2 + 3x_3 \\ 4x_1 + 5x_2 + 6x_3 \end{bmatrix}_{2 \times 1}$$

$$= \begin{bmatrix} \underline{\alpha}_1^T \\ \underline{\alpha}_2^T \end{bmatrix} \underline{x}$$

$$= \begin{bmatrix} \underline{\alpha}_1^T \underline{x} \\ \underline{\alpha}_2^T \underline{x} \end{bmatrix} = \begin{bmatrix} \langle \underline{\alpha}_1, \underline{x} \rangle \\ \langle \underline{\alpha}_2, \underline{x} \rangle \end{bmatrix}$$

□ Note: $\underline{y}_{m \times 1} = A_{m \times n} \underline{x}_{n \times 1}$

□ In general:

$$\underline{y} = A \underline{x} = \begin{bmatrix} \underline{\alpha}_1^T \\ \vdots \\ \underline{\alpha}_m^T \end{bmatrix} \underline{x} = \begin{bmatrix} \underline{\alpha}_1^T \underline{x} \\ \vdots \\ \underline{\alpha}_m^T \underline{x} \end{bmatrix}$$

$$y_k = \underline{\alpha}_k^T \underline{x} \quad \text{for } k=1, \dots, m$$

Dot Product View.

Alternatively e.g.: Lin. Combo of Cols. of A
View

$$\begin{aligned} \underbrace{\begin{bmatrix} 1 & 2 & 3 \\ 4 & 5 & 6 \end{bmatrix}}_{\substack{\underline{A} \\ 2 \times 3}} \underbrace{\begin{bmatrix} x_1 \\ x_2 \\ x_3 \end{bmatrix}}_{\substack{\underline{x} \\ 3 \times 1}} &= \begin{bmatrix} 1x_1 + 2x_2 + 3x_3 \\ 4x_1 + 5x_2 + 6x_3 \end{bmatrix}_{2 \times 1} \\ &= \begin{bmatrix} 1x_1 \\ 4x_1 \end{bmatrix} + \begin{bmatrix} 2x_2 \\ 5x_2 \end{bmatrix} + \begin{bmatrix} 3x_3 \\ 6x_3 \end{bmatrix} \\ &= x_1 \begin{bmatrix} 1 \\ 4 \end{bmatrix} + x_2 \begin{bmatrix} 2 \\ 5 \end{bmatrix} + x_3 \begin{bmatrix} 3 \\ 6 \end{bmatrix} \\ &= x_1 \underline{a}_1 + x_2 \underline{a}_2 + x_3 \underline{a}_3 \end{aligned}$$

□ In general

$$\begin{aligned} A = [\underline{a}_1 \ \dots \ \underline{a}_n]_{m \times n} &\rightarrow A\underline{x} = x_1 \underline{a}_1 + \dots + x_n \underline{a}_n \\ \underline{a}_i \in \mathbb{R}^m & \\ &= \sum_{i=1}^n x_i \underline{a}_i \end{aligned}$$

Column-Linear-Combo of Columns of A
View of $A\underline{x}$.

Matrix Multiplication

$$C_{m \times n} = A_{m \times p} B_{p \times n}$$

1) Inner Product View

$$A = [\underline{a}_1, \dots, \underline{a}_\ell, \dots, \underline{a}_p] = \begin{bmatrix} \underline{\alpha}_1^T \\ \vdots \\ \underline{\alpha}_\ell^T \\ \vdots \\ \underline{\alpha}_m^T \end{bmatrix}$$

$$B = [\underline{b}_1, \dots, \underline{b}_\ell, \dots, \underline{b}_n] = \begin{bmatrix} \underline{\beta}_1^T \\ \vdots \\ \underline{\beta}_\ell^T \\ \vdots \\ \underline{\beta}_p^T \end{bmatrix}$$

Inner
Product
View

$$C = AB = \begin{bmatrix} \underline{\alpha}_1^T \\ \vdots \\ \underline{\alpha}_\ell^T \\ \vdots \\ \underline{\alpha}_m^T \end{bmatrix} [\underline{b}_1 \dots \underline{b}_\ell \dots \underline{b}_n]$$

$$= \begin{bmatrix} \underline{\alpha}_1^T \underline{b}_1 & \dots & \underline{\alpha}_1^T \underline{b}_\ell & \dots & \underline{\alpha}_1^T \underline{b}_n \\ \vdots & & \vdots & & \vdots \\ \underline{\alpha}_\ell^T \underline{b}_1 & \dots & \underline{\alpha}_\ell^T \underline{b}_\ell & \dots & \underline{\alpha}_\ell^T \underline{b}_n \\ \vdots & & \vdots & & \vdots \\ \underline{\alpha}_m^T \underline{b}_1 & \dots & \underline{\alpha}_m^T \underline{b}_\ell & \dots & \underline{\alpha}_m^T \underline{b}_n \end{bmatrix}$$

$$C_{k\ell} = \underline{\alpha}_k^T \underline{b}_\ell$$

$$k \in \{1, \dots, m\}$$

$$\ell \in \{1, \dots, n\}$$

eg. $C = \underbrace{\begin{bmatrix} 1 & 2 & 3 \\ 4 & 5 & 6 \end{bmatrix}}_A \underbrace{\begin{bmatrix} 0 & 3 \\ 1 & 4 \\ 2 & 5 \end{bmatrix}}_B = \begin{bmatrix} 1 \cdot 0 + 2 \cdot 1 + 3 \cdot 2 & 1 \cdot 3 + 2 \cdot 4 + 3 \cdot 5 \\ 4 \cdot 0 + 5 \cdot 1 + 6 \cdot 2 & 4 \cdot 3 + 5 \cdot 4 + 6 \cdot 5 \end{bmatrix}$

2) Cols. of C viewed as lin. combos. of cols of A .

$$C = AB$$

Consider: $\underline{c}_1 = A\underline{b}_1 \dots \underline{c}_2 = A\underline{b}_2 \dots \underline{c}_n = A\underline{b}_n$

$$\begin{aligned} [\underline{c}_1 \dots \underline{c}_2 \dots \underline{c}_n] &= [A\underline{b}_1 \dots A\underline{b}_2 \dots A\underline{b}_n] \quad \text{lin. combo. of cols of } A \\ &= A [\underbrace{\underline{b}_1 \dots \underline{b}_2 \dots \underline{b}_n}_B] \end{aligned}$$

$$\underline{c}_2 = A\underline{b}_2 = [\underline{a}_1 \dots \underline{a}_r \dots \underline{a}_p] \begin{bmatrix} b_{r2} \\ \vdots \\ b_{p2} \end{bmatrix}$$

$$= b_{r2} \underline{a}_1 + \dots + b_{p2} \underline{a}_p$$

... ?

eg. $C = \underbrace{\begin{bmatrix} 1 & 2 & 3 \\ 4 & 5 & 6 \end{bmatrix}}_A \underbrace{\begin{bmatrix} 0 & 3 \\ 1 & 4 \\ 2 & 5 \end{bmatrix}}_B$

$$= \left[\underbrace{0 \begin{bmatrix} 1 \\ 4 \end{bmatrix} + 1 \begin{bmatrix} 2 \\ 5 \end{bmatrix} + 2 \begin{bmatrix} 3 \\ 6 \end{bmatrix}}_{\underline{c}_1 \text{ (1st col of } C)} \quad \underbrace{3 \begin{bmatrix} 1 \\ 4 \end{bmatrix} + 4 \begin{bmatrix} 2 \\ 5 \end{bmatrix} + 5 \begin{bmatrix} 3 \\ 6 \end{bmatrix}}_{\underline{c}_2} \right]$$

3) Rows of C viewed as lin. combos. of the rows of B .

$$C = AB$$

$$\begin{bmatrix} \underline{\sigma}_1^T \\ \vdots \\ \underline{\sigma}_k^T \\ \vdots \\ \underline{\sigma}_m^T \end{bmatrix} = \begin{bmatrix} \underline{\sigma}_1^T \\ \vdots \\ \underline{\sigma}_k^T \\ \vdots \\ \underline{\sigma}_m^T \end{bmatrix} B = \begin{bmatrix} \underline{\sigma}_1^T B \\ \vdots \\ \underline{\sigma}_k^T B \\ \vdots \\ \underline{\sigma}_m^T B \end{bmatrix}$$

$$\underline{\sigma}_k^T = k^{\text{th}} \text{ row of } C$$

$$\underline{\sigma}_k^T = \underline{\sigma}_k^T B = [\underline{a}_{k1} \dots \underline{a}_{kr} \dots \underline{a}_{kp}] \begin{bmatrix} \underline{\beta}_1^T \\ \vdots \\ \underline{\beta}_r^T \\ \vdots \\ \underline{\beta}_p^T \end{bmatrix}$$

$$\begin{aligned} \underline{\sigma}_k^T &= \underline{a}_{k1} \underline{\beta}_1^T + \dots + \underline{a}_{kr} \underline{\beta}_r^T + \underline{a}_{kp} \underline{\beta}_p^T \\ &= \sum_{r=1}^p \underline{a}_{kr} \underline{\beta}_r^T \end{aligned}$$

e.g. $C = \underbrace{\begin{bmatrix} 1 & 2 & 3 \\ 4 & 5 & 6 \end{bmatrix}}_A \underbrace{\begin{bmatrix} 0 & 3 \\ 1 & 4 \\ 2 & 5 \end{bmatrix}}_B$

$$= \begin{bmatrix} [1[0 \ 3] + 2[1 \ 4] + 3[2 \ 5]] \\ [4[0 \ 3] + 5[1 \ 4] + 6[2 \ 5]] \end{bmatrix}$$

- 4th View

Detour: **Outer Product** (Dyadic Product)

$$\underline{a} = \begin{bmatrix} 1 \\ 2 \\ 3 \end{bmatrix}_{3 \times 1} \quad \underline{b} = \begin{bmatrix} 4 \\ 5 \end{bmatrix}_{2 \times 1}$$

$$\underline{a}\underline{b}^T = \begin{bmatrix} 1 \\ 2 \\ 3 \end{bmatrix}_{3 \times 1} \begin{bmatrix} 4 & 5 \end{bmatrix}_{1 \times 2} = \begin{bmatrix} 4 & 5 \\ 8 & 10 \\ 12 & 15 \end{bmatrix}_{3 \times 2}$$

$$= \begin{bmatrix} 1 \begin{bmatrix} 4 & 5 \end{bmatrix} \\ 2 \begin{bmatrix} 4 & 5 \end{bmatrix} \\ 3 \begin{bmatrix} 4 & 5 \end{bmatrix} \end{bmatrix} = \begin{bmatrix} 4 \begin{bmatrix} 1 \\ 2 \\ 3 \end{bmatrix} & 5 \begin{bmatrix} 1 \\ 2 \\ 3 \end{bmatrix} \end{bmatrix} = \underline{a} [\underline{b}_1 \dots \underline{b}_n]$$

→ In general:

$$4) \quad \underline{a}\underline{b}^T = \underline{a} [\underline{b}_1 \dots \underline{b}_n] = [\underline{a}\underline{b}_1 \dots \underline{a}\underline{b}_n]_{m \times n}$$

only 1 indep. col. All others are scalar multiples.

Now, $C = AB$ viewed as sum of outer products of cols. of A & rows of B .

$$C = [\underline{a}_1 \dots \underline{a}_e \dots \underline{a}_p] \begin{bmatrix} \underline{\beta}_1^T \\ \vdots \\ \underline{\beta}_e^T \\ \vdots \\ \underline{\beta}_p^T \end{bmatrix} \quad \underline{\beta}_i \in \mathbb{R}^n$$

$\underline{a}_e \in \mathbb{R}^m$

$$= \underline{a}_1 \underline{\beta}_1^T + \dots + \underline{a}_e \underline{\beta}_e^T + \dots + \underline{a}_p \underline{\beta}_p^T \quad \begin{matrix} \underline{a}_e \underline{\beta}_e^T \\ m \times 1 \quad 1 \times n \end{matrix}$$

$$C = \sum_{e=1}^p \underline{a}_e \underline{\beta}_e^T$$

4) cont'd

e.g. $C = \underbrace{\begin{bmatrix} 1 & 2 & 3 \\ 4 & 5 & 6 \end{bmatrix}}_A \underbrace{\begin{bmatrix} 0 & 3 \\ 1 & 4 \\ 2 & 5 \end{bmatrix}}_B$

$$= \begin{bmatrix} 1 \\ 4 \end{bmatrix} \begin{bmatrix} 0 & 3 \end{bmatrix} + \begin{bmatrix} 2 \\ 5 \end{bmatrix} \begin{bmatrix} 1 & 4 \end{bmatrix} + \begin{bmatrix} 3 \\ 6 \end{bmatrix} \begin{bmatrix} 2 & 5 \end{bmatrix}$$

=

Concept	Symbolic notation	Index (Einstein) notation
Vector-matrix product	$y = Ax$ wikipedia	$y_i = \sum_j a_{ij} x_j$ or $y_i = a_{ij} x_j$ brown
Inner product	$x^T y$ wikipedia	$\sum_i x_i y_i = x_i y_i$ brown
Quadratic form	$x^T A x$ wikipedia	$\sum_{i,j} a_{ij} x_i x_j = a_{ij} x_i x_j$ brown
Trace/Frobenius	$\text{tr}(A^T B)$ math.uwaterloo	$\sum_{i,j} a_{ij} b_{ij}$ brown
Jacobian of linear map	$\frac{\partial(Ax)}{\partial x} = A$ (numerator layout) wikipedia	$\frac{\partial y_i}{\partial x_k} = a_{ik}$ so the Jacobian has entries a_{ik} wikipedia



3 Matrix Multiplication

Definition 3 Let \mathbf{A} be $m \times n$, and \mathbf{B} be $n \times p$, and let the product \mathbf{AB} be

$$\mathbf{C} = \mathbf{AB} \quad (3)$$

then \mathbf{C} is a $m \times p$ matrix, with element (i, j) given by

$$c_{ij} = \sum_{k=1}^n a_{ik} b_{kj} \quad (4)$$

for all $i = 1, 2, \dots, m$, $j = 1, 2, \dots, p$.

Proposition 1 Let \mathbf{A} be $m \times n$, and \mathbf{x} be $n \times 1$, then the typical element of the product

$$\mathbf{z} = \mathbf{Ax} \quad (5)$$

is given by

$$z_i = \sum_{k=1}^n a_{ik} x_k \quad (6)$$

for all $i = 1, 2, \dots, m$. Similarly, let \mathbf{y} be $m \times 1$, then the typical element of the product

$$\mathbf{z}^T = \mathbf{y}^T \mathbf{A} \quad (7)$$

is given by

$$z_i = \sum_{k=1}^n a_{ki} y_k = (A^T)_{ik} y_k \quad (8)$$

for all $i = 1, 2, \dots, n$. Finally, the scalar resulting from the product

$$\alpha = \mathbf{y}^T \mathbf{Ax} \quad (9)$$

is given by

$$\alpha = \sum_{j=1}^m \sum_{k=1}^n a_{jk} y_j x_k \quad (10)$$

Proof: These are merely direct applications of Definition 3. q.e.d.

$$\Rightarrow \begin{aligned} \mathbf{z} &= A^T \mathbf{y} \\ \mathbf{z}^T &= \mathbf{y}^T A \end{aligned}$$

Proposition 2 Let \mathbf{A} be $m \times n$, and \mathbf{B} be $n \times p$, and let the product \mathbf{AB} be

$$\mathbf{C} = \mathbf{AB} \quad (11)$$

then

$$\mathbf{C}^T = \mathbf{B}^T \mathbf{A}^T \quad (12)$$

Proof: The typical element of \mathbf{C} is given by

$$c_{ij} = \sum_{k=1}^n a_{ik} b_{kj} \quad (13)$$

By definition, the typical element of \mathbf{C}^T , say d_{ij} , is given by

$$d_{ij} = c_{ji} = \sum_{k=1}^n a_{jk} b_{ki} = \sum_{k=1}^n b_{ki} a_{jk} \quad (14)$$

Hence,

$$\mathbf{C}^T = \mathbf{B}^T \mathbf{A}^T = \sum_{k=1}^n (\mathbf{B}^T)_{ik} (\mathbf{A}^T)_{kj} \quad (15)$$

q.e.d.



5 Matrix Differentiation

In the following discussion I will differentiate matrix quantities with respect to the elements of the referenced matrices. Although no new concept is required to carry out such operations, the element-by-element calculations involve cumbersome manipulations and, thus, it is useful to derive the necessary results and have them readily available ².

Convention 3

Let

$$\mathbf{y} = \psi(\mathbf{x}), \quad (23)$$

where \mathbf{y} is an m -element vector, and \mathbf{x} is an n -element vector. The symbol

$$\psi(x) : \mathbb{R}^n \rightarrow \mathbb{R}^m$$

$$\frac{\partial \mathbf{y}}{\partial \mathbf{x}} = \begin{bmatrix} \frac{\partial y_1}{\partial x_1} & \frac{\partial y_1}{\partial x_2} & \cdots & \frac{\partial y_1}{\partial x_n} \\ \frac{\partial y_2}{\partial x_1} & \frac{\partial y_2}{\partial x_2} & \cdots & \frac{\partial y_2}{\partial x_n} \\ \vdots & \vdots & & \vdots \\ \frac{\partial y_m}{\partial x_1} & \frac{\partial y_m}{\partial x_2} & \cdots & \frac{\partial y_m}{\partial x_n} \end{bmatrix} \quad (24)$$

will denote the $m \times n$ matrix of first-order partial derivatives of the transformation from \mathbf{x} to \mathbf{y} . Such a matrix is called the Jacobian matrix of the transformation $\psi()$.

Notice that if \mathbf{x} is actually a scalar in Convention 3 then the resulting Jacobian matrix is a $m \times 1$ matrix; that is, a single column (a vector). On the other hand, if \mathbf{y} is actually a scalar in Convention 3 then the resulting Jacobian matrix is a $1 \times n$ matrix; that is, a single row (the transpose of a vector).

Almost—more precisely, a Jacobian is the $m \times n$ matrix of first-order partial derivatives of a vector-valued map $\psi: \mathbb{R}^n \rightarrow \mathbb{R}^m$, arranged with the i -th row equal to the gradient of the i -th output component and the j -th column giving sensitivities with respect to x_j across outputs. Beyond being “elementwise derivatives,” the Jacobian represents the linear map (the differential) that best approximates ψ near a point: $\psi(x) \approx \psi(x_0) + J\psi(x_0)(x - x_0)$ for x near x_0 . When $m=1$, the Jacobian reduces to the row form of the gradient; when $n=m$ and one takes its determinant, that determinant is the “Jacobian” used in change of variables. [wikipedia +2](#)

Proposition 5 *Let*

$$\mathbf{y} = \mathbf{A}\mathbf{x} \quad (25)$$

where \mathbf{y} is $m \times 1$, \mathbf{x} is $n \times 1$, \mathbf{A} is $m \times n$, and \mathbf{A} does not depend on \mathbf{x} , then

$$\frac{\partial \mathbf{y}}{\partial \mathbf{x}} = \mathbf{A} \quad (26)$$

Proof: Since the i th element of \mathbf{y} is given by

$$y_i = \sum_{k=1}^n a_{ik} x_k \quad (27)$$

it follows that

$$\frac{\partial y_i}{\partial x_j} = a_{ij} \quad (28)$$

for all $i = 1, 2, \dots, m$, $j = 1, 2, \dots, n$. Hence

$$\frac{\partial \mathbf{y}}{\partial \mathbf{x}} = \mathbf{A} \quad (29)$$

q.e.d.

Proposition 6 *Let*

$$\mathbf{y} = \mathbf{A}\mathbf{x} \quad (30)$$

where \mathbf{y} is $m \times 1$, \mathbf{x} is $n \times 1$, \mathbf{A} is $m \times n$, and \mathbf{A} does not depend on \mathbf{x} , as in Proposition 5. Suppose that \mathbf{x} is a function of the vector \mathbf{z} , while \mathbf{A} is independent of \mathbf{z} . Then

$$\frac{\partial \mathbf{y}}{\partial \mathbf{z}} = \mathbf{A} \frac{\partial \mathbf{x}}{\partial \mathbf{z}} \quad (31)$$

Proof: Since the i th element of \mathbf{y} is given by

$$y_i = \sum_{k=1}^n a_{ik} x_k \quad (32)$$

for all $i = 1, 2, \dots, m$, it follows that

$$\frac{\partial y_i}{\partial z_j} = \sum_{k=1}^n a_{ik} \frac{\partial x_k}{\partial z_j} \quad (33)$$

but the right hand side of the above is simply element (i, j) of $\mathbf{A} \frac{\partial \mathbf{x}}{\partial \mathbf{z}}$. Hence

$$\frac{\partial \mathbf{y}}{\partial \mathbf{z}} = \frac{\partial \mathbf{y}}{\partial \mathbf{x}} \frac{\partial \mathbf{x}}{\partial \mathbf{z}} = \mathbf{A} \frac{\partial \mathbf{x}}{\partial \mathbf{z}} \quad (34)$$

q.e.d.

Chain rule holds

Proposition 7 *Let the scalar α be defined by*

$$\alpha = \mathbf{y}^\top \mathbf{A} \mathbf{x} \quad (35)$$

where \mathbf{y} is $\mathbf{m} \times 1$, \mathbf{x} is $\mathbf{n} \times 1$, \mathbf{A} is $\mathbf{m} \times \mathbf{n}$, and \mathbf{A} is independent of \mathbf{x} and \mathbf{y} , then

$$\frac{\partial \alpha}{\partial \mathbf{x}} = \mathbf{y}^\top \mathbf{A} \quad (36)$$

and

$$\frac{\partial \alpha}{\partial \mathbf{y}} = \mathbf{x}^\top \mathbf{A}^\top \quad (37)$$

Proof: Define

$$\mathbf{w}^\top = \mathbf{y}^\top \mathbf{A} \quad (38)$$

and note that

$$\alpha = \mathbf{w}^\top \mathbf{x} \quad (39)$$

Hence, by Proposition 5 we have that

$$\frac{\partial \alpha}{\partial \mathbf{x}} = \mathbf{w}^\top = \mathbf{y}^\top \mathbf{A} \quad (40)$$

which is the first result. Since α is a scalar, we can write

$$\alpha = \alpha^\top = \mathbf{x}^\top \mathbf{A}^\top \mathbf{y} \quad (41)$$

and applying Proposition 5 as before we obtain

$$\frac{\partial \alpha}{\partial \mathbf{y}} = \mathbf{x}^\top \mathbf{A}^\top \quad (42)$$

q.e.d.

HW 0 Answers...

Proposition 8 For the special case in which the scalar α is given by the quadratic form

$$\alpha = \mathbf{x}^T \mathbf{A} \mathbf{x} \quad (43)$$

where \mathbf{x} is $n \times 1$, \mathbf{A} is $n \times n$, and \mathbf{A} does not depend on \mathbf{x} , then

$$\frac{\partial \alpha}{\partial \mathbf{x}} = \mathbf{x}^T (\mathbf{A} + \mathbf{A}^T) \quad (44)$$

Proof: By definition

$$\alpha = \sum_{j=1}^n \sum_{i=1}^n a_{ij} x_i x_j \quad (45)$$

Def 3
Prop 1

Differentiating with respect to the k th element of \mathbf{x} we have

$$\frac{\partial \alpha}{\partial x_k} = \sum_{i=1}^n a_{ki} x_i + \sum_{j=1}^n a_{jk} x_j \quad (46)$$

for all $k = 1, 2, \dots, n$, and consequently,

$$\frac{\partial \alpha}{\partial \mathbf{x}} = \mathbf{x}^T \mathbf{A}^T + \mathbf{x}^T \mathbf{A} = \mathbf{x}^T (\mathbf{A}^T + \mathbf{A}) \quad (47)$$

q.e.d.

Proposition 9 For the special case where \mathbf{A} is a symmetric matrix and

$$\alpha = \mathbf{x}^T \mathbf{A} \mathbf{x} \quad (48)$$

where \mathbf{x} is $n \times 1$, \mathbf{A} is $n \times n$, and \mathbf{A} does not depend on \mathbf{x} , then

$$\frac{\partial \alpha}{\partial \mathbf{x}} = 2\mathbf{x}^T \mathbf{A} \quad (49)$$

Proof: This is an obvious application of Proposition 8. q.e.d.